remove stdpp dependency

theories/instantiation_properties.v
@@ -1,15 +1,352 @@
 (* Properties of instantiation spec *)
-(* Taken from the Iris branch, so some dependencies on stdpp *)
 
-Require Import Coq.Program.Equality.
 From mathcomp Require Import ssreflect eqtype seq ssrbool ssrfun.
+Require Import Coq.Program.Equality List NArith.
 Require Export instantiation_spec.
-From stdpp Require Import list fin_maps gmap.
-Require Export stdpp_aux.
 Require Export type_preservation type_progress.
-  
+
+
+Notation "l !! n" := (List.nth_error l n) (at level 10).
+
 Section module_typing_det.
-  
+
+Lemma list_eq {T: Type} (l1 l2: list T):
+  (forall i, List.nth_error l1 i = List.nth_error l2 i) -> l1 = l2.
+Proof.
+  move: l1 l2.
+  induction l1; destruct l2 => //=; move => H; try by specialize (H 0).
+  f_equal.
+  - specialize (H 0); by injection H.
+  - apply IHl1; move => i.
+    by specialize (H (S i)).
+Qed.
+
+Lemma Forall2_length {T1 T2: Type} (f: T1 -> T2 -> Prop) l1 l2:
+  List.Forall2 f l1 l2 ->
+  length l1 = length l2.
+Proof.
+  move: l1 l2.
+  induction l1; destruct l2 => //=; move => H; inversion H; subst; clear H.
+  f_equal; by apply IHl1.
+Qed.
+
+Lemma Forall_lookup {T: Type} (P: T -> Prop) l i x:
+  List.Forall P l ->
+  List.nth_error l i = Some x ->
+  P x.
+Proof.
+  move: l i x.
+  induction l; destruct i => //=; move => x Hall Hnth.
+  - injection Hnth as ->.
+    by inversion Hall.
+  - eapply IHl; eauto => //.
+    by inversion Hall.
+Qed.
+
+Lemma Forall_spec {T: Type} (P: T -> Prop) (l: list T):
+  (forall n x, List.nth_error l n = Some x -> P x) ->
+  Forall P l.
+Proof.
+  induction l; move => Hspec => //.
+  constructor.
+  - by eapply (Hspec 0 a).
+  - apply IHl.
+    move => n x Hnth.
+    by apply (Hspec (S n) x).
+Qed.
+
+Lemma Forall2_lookup {T1 T2: Type} (f: T1 -> T2 -> Prop) l1 l2 i x:
+  List.Forall2 f l1 l2 ->
+  List.nth_error l1 i = Some x ->
+  exists y, List.nth_error l2 i = Some y /\ f x y.
+Proof.
+  move: l1 l2 i x.
+  induction l1; destruct l2, i => //=; move => x Hall2 Hnth; try by inversion Hall2.
+  - injection Hnth as ->. eexists; split => //.
+    by inversion Hall2.
+  - apply IHl1 => //.
+    by inversion Hall2.
+Qed.
+
+Lemma Forall2_function_eq_cond {T1 T2: Type} (P: T1 -> Prop) (f g: T1 -> T2 -> Prop) l1 l2 l3:
+  List.Forall P l1 ->
+  List.Forall2 f l1 l2 ->
+  List.Forall2 g l1 l3 ->
+  (forall x y z, P x -> f x y -> g x z -> y = z) ->
+  l2 = l3.
+Proof.
+  move => Hall Hall2f Hall2g Heq.
+  apply list_eq.
+  move => i.
+  destruct (List.nth_error l1 i) eqn:Hnth.
+  { eapply Forall_lookup in Hall; eauto => //.
+    eapply Forall2_lookup in Hall2f as [y [Hnth1 Hf]]; eauto => //.
+    eapply Forall2_lookup in Hall2g as [z [Hnth2 Hg]]; eauto => //.
+    rewrite Hnth1 Hnth2; f_equal.
+    by eapply Heq; eauto.
+  }
+  { apply Forall2_length in Hall2f.
+    apply Forall2_length in Hall2g.
+    apply List.nth_error_None in Hnth.
+    specialize (List.nth_error_None l2 i) as [_ Hnone1].
+    rewrite Hnone1; last by lias.
+    symmetry. rewrite -> List.nth_error_None. by lias.
+  }
+Qed.
+
+Lemma Forall2_function_eq {T1 T2: Type} (f g: T1 -> T2 -> Prop) l1 l2 l3:
+  List.Forall2 f l1 l2 ->
+  List.Forall2 g l1 l3 ->
+  (forall x y z, f x y -> g x z -> y = z) ->
+  l2 = l3.
+Proof.
+  move => Hall2f Hall2g Heq.
+  eapply Forall2_function_eq_cond with (P := fun _ => True) in Hall2g; eauto.
+  clear. by induction l1; constructor.
+Qed.
+
+Lemma Forall2_all2: forall {A B: Type} (R : A -> B -> bool) (l1 : seq.seq A) (l2 : seq.seq B),
+    List.Forall2 R l1 l2 <-> all2 R l1 l2.
+Proof.
+  move => A B R l1.
+  split.
+  - move: l2.
+    induction l1; move => l2 HForall2.
+    * by inversion HForall2.
+    * inversion HForall2; subst.
+      specialize (IHl1 l' H3).
+      apply/andP. split => //.
+  - move: l2.
+    induction l1; move => l2 Hall2.
+    * inversion Hall2. by destruct l2 => //.
+    * inversion Hall2. destruct l2 => //.
+      move/andP in H0. destruct H0.
+      specialize (IHl1 l2 H0).
+      apply Forall2_cons => //.
+Qed.
+
+Lemma all2_and: forall A B (f g h : A -> B -> bool) l1 l2,
+  (forall a b, f a b = (g a b) && (h a b)) -> 
+  all2 g l1 l2 /\ all2 h l1 l2 -> 
+  all2 f l1 l2.
+Proof.
+  move => A B f g h l1 l2 Hand [Hg Hh].
+  apply all2_spec; first by apply all2_size in Hg.
+  move => n x y Hnth1 Hnth2.
+  eapply all2_projection in Hg; eauto.
+  eapply all2_projection in Hh; eauto.
+  rewrite Hand; by lias.
+Qed.
+
+Lemma Forall2_nth_error: forall A B R (l1 : seq.seq A) (l2 : seq.seq B) n m k,
+    List.Forall2 R l1 l2 ->
+    List.nth_error l1 n = Some m ->
+    List.nth_error l2 n = Some k ->
+    R m k.
+Proof.
+  move => A B R l1 l2 n m k HForall2 Hnth1 Hnth2.
+  eapply Forall2_lookup in Hnth1; eauto.
+  destruct Hnth1 as [y [Hnth2' HR]].
+  rewrite Hnth2' in Hnth2; by injection Hnth2 as ->.
+Qed.
+
+Lemma Forall2_spec: forall A B (R : A -> B -> Prop) (l1 : seq.seq A) (l2 : seq.seq B),
+    List.length l1 = List.length l2 -> 
+    (forall n m k,
+    List.nth_error l1 n = Some m -> 
+    List.nth_error l2 n = Some k ->
+    R m k) ->
+    List.Forall2 R l1 l2.
+Proof.
+  move => A B R l1.
+  induction l1; move => l2 Hlen Hlookup; destruct l2 => //; simpl in *.
+  constructor.
+  - by apply (Hlookup 0 a b).
+  - apply IHl1; first by lias.
+    move => i x y Hl1 Hl2.
+    by eapply (Hlookup (S i)) => //.
+Qed.
+
+Lemma nth_error_same_length_list:
+  forall (A B : Type) (l1 : seq.seq A) (l2 : seq.seq B) (i : nat) (m : A),
+     length l1 = length l2 ->
+     nth_error l1 i = Some m -> 
+     exists n, nth_error l2 i = Some n.
+Proof.
+  move => A B l1 l2 i m Hlen Hl1.
+  apply nth_error_Some_length in Hl1.
+  rewrite Hlen in Hl1.
+  apply nth_error_Some in Hl1.
+  by destruct (l2 !! i) => //; eexists.
+Qed.
+
+Fixpoint imap_aux {T1 T2: Type} (f: nat -> T1 -> T2) (l: list T1) (i: nat) : list T2 :=
+  match l with
+  | [::] => [::]
+  | e :: l' => (f i e) :: imap_aux f l' (S i)
+  end.
+
+Definition imap {T1 T2: Type} (f: nat -> T1 -> T2) l := imap_aux f l 0.
+
+Lemma imap_extend_aux {T1 T2: Type} (f: nat -> T1 -> T2) l e j:
+  imap_aux f (app l [:: e]) j = app (imap_aux f l j) [:: f (length l + j) e].
+Proof.
+  move: j.
+  induction l => //=; move => j.
+  f_equal. rewrite (IHl (S j)).
+  repeat f_equal.
+  by lias.
+Qed.
+
+Lemma imap_extend {T1 T2: Type} (f: nat -> T1 -> T2) l e:
+  imap f (app l [:: e]) = app (imap f l) [:: f (length l) e].
+Proof.
+  unfold imap.
+  rewrite (imap_extend_aux f l e 0).
+  repeat f_equal.
+  by lias.
+Qed.
+
+Lemma imap_length_aux {T1 T2: Type} (f: nat -> T1 -> T2) l j:
+  length (imap_aux f l j) = length l.
+Proof.
+  move: j.
+  induction l => //=; move => j.
+  f_equal; by apply IHl.
+Qed.
+
+Lemma imap_length {T1 T2: Type} (f: nat -> T1 -> T2) l:
+  length (imap f l) = length l.
+Proof.
+  by apply (imap_length_aux f l 0).
+Qed.
+
+Lemma list_lookup_imap_aux {T1 T2: Type} (f: nat -> T1 -> T2) l i j:
+  List.nth_error (imap_aux f l j) i = option_map (f (i + j)) (List.nth_error l i).
+Proof.
+  move: l i j.
+  induction l; destruct i; move => j => //=.
+  specialize (IHl i (S j)).
+  rewrite IHl; repeat f_equal. by lias.
+Qed.
+
+Lemma list_lookup_imap {T1 T2: Type} (f: nat -> T1 -> T2) l i:
+  List.nth_error (imap f l) i = option_map (f i) (List.nth_error l i).
+Proof.
+  unfold imap.
+  rewrite -> (list_lookup_imap_aux f l i 0).
+  by rewrite PeanoNat.Nat.add_0_r.
+Qed.
+
+Lemma repeat_lookup {T: Type} (x: T) n i:
+  i < n ->
+  List.nth_error (List.repeat x n) i = Some x.
+Proof.
+  move: i.
+  induction n; destruct i => //=; move => H; try by inversion H.
+  by apply IHn; lias.
+Qed.
+
+Lemma repeat_lookup_Some {T: Type} (x y: T) n i:
+  List.nth_error (List.repeat x n) i = Some y ->
+  x = y /\ i < n.
+Proof.
+  move: i.
+  induction n; destruct i => //=; move => H; try by inversion H; lias.
+  apply IHn in H as [-> Hlt].
+  split; by lias.
+Qed.
+
+Lemma NoDup_alt {T: Type} (l: list T):
+  (forall i j x, l !! i = Some x -> l !! j = Some x -> i = j) -> List.NoDup l.
+Proof.
+  induction l; move => H => //; try by constructor.
+  constructor.
+  - move => Hin.
+    apply List.In_nth_error in Hin as [n Hnth].
+    specialize (H 0 (S n) a); simpl in H.
+    by apply H in Hnth => //.
+  - apply IHl.
+    move => i j x Hnth1 Hnth2.
+    specialize (H (S i) (S j) x); simpl in H.
+    by apply H in Hnth1; lias.
+Qed.
+    
+Definition gen_index offset len : list nat :=
+  imap (fun i x => i+offset+x) (List.repeat 0 len).
+
+Lemma gen_index_lookup offset len k:
+  k < len ->
+  (gen_index offset len) !! k = Some (offset + k).
+Proof.
+  move => Hlen.
+  unfold gen_index.
+  rewrite list_lookup_imap => /=.
+  eapply repeat_lookup with (x := 0) in Hlen.
+  rewrite Hlen.
+  simpl.
+  f_equal.
+  by lias.
+Qed.
+
+Lemma gen_index_lookup_Some n l i x:
+  (gen_index n l) !! i = Some x ->
+  x = n + i /\ i < l.
+Proof.
+  unfold gen_index.
+  move => Hl.
+  rewrite list_lookup_imap in Hl.
+  destruct (List.repeat _ _ !! i) eqn: Hrl => //.
+  simpl in Hl.
+  inversion Hl; subst; clear Hl.
+  apply repeat_lookup_Some in Hrl as [<- ?].
+  by lias.
+Qed.
+ 
+Lemma gen_index_NoDup n l:
+  List.NoDup (gen_index n l).
+Proof.
+  apply NoDup_alt.
+  move => i j x Hli Hlj.
+  apply gen_index_lookup_Some in Hli as [-> ?].
+  apply gen_index_lookup_Some in Hlj as [? ?].
+  by lias.
+Qed.
+
+Lemma gen_index_length n len:
+  length (gen_index n len) = len.
+Proof.
+  unfold gen_index.
+  rewrite imap_length.
+  by rewrite List.repeat_length.
+Qed.
+
+Lemma gen_index_extend offset len:
+  gen_index offset (len+1) = gen_index offset len ++ [::offset+len].
+Proof.
+  unfold gen_index.
+  rewrite List.repeat_app imap_extend List.repeat_length => /=.
+  do 2 f_equal.
+  by lias.
+Qed.
+
+Lemma gen_index_len offset len:
+  length (gen_index offset len) = len.
+Proof.
+  unfold gen_index.
+  rewrite imap_length.
+  by rewrite repeat_length.
+Qed.
+
+Lemma gen_index_in n i offset len:
+  (gen_index offset len) !! n = Some i  ->
+  i < offset + len.
+Proof.
+  move => H.
+  apply gen_index_lookup_Some in H as [-> Hlt].
+  by lias.
+Qed.
+
 Lemma module_typing_det_import_aux m it1 et1 it2 et2:
   module_typing m it1 et1 ->
   module_typing m it2 et2 ->
@@ -22,49 +359,12 @@ Proof.
   destruct Hmt2 as [fts2 [gts2 [Hmft2 [Hmtt2 [Hmmt2 [Hmgt2 [Hmet2 [Hmdt2 [Hmst2 [Hmimt2 Hmext2]]]]]]]]]].
   
   clear - Hmimt1 Hmimt2.
-  apply list_eq.
-  move => i.
-  rewrite -> Forall2_lookup in Hmimt1.
-  specialize (Hmimt1 i).
-  rewrite -> Forall2_lookup in Hmimt2.
-  specialize (Hmimt2 i).    
-  destruct (it1 !! i) eqn:Hitl1; destruct (it2 !! i) eqn:Hitl2; inversion Hmimt1; inversion Hmimt2; subst => //=.
-  - rewrite <- H in H2.
-    inversion H2; subst; clear H2.
-    destruct x; simpl in *.
-    unfold module_import_typing in *.
-    destruct imp_desc; simpl in *; destruct e; destruct e0 => //.
-    { (* func *)
-      move/andP in H1; destruct H1.
-      move/andP in H4; destruct H4.
-      destruct (nth_error mod_types n) => //.
-      move/eqP in H1.
-      move/eqP in H3.
-      by subst.
-    }
-    { (* table *)
-      move/andP in H1; destruct H1.
-      move/andP in H4; destruct H4.
-      move/eqP in H0.
-      move/eqP in H2.
-      by subst.
-    }
-    { (* memory *)
-      move/andP in H1; destruct H1.
-      move/andP in H4; destruct H4.
-      move/eqP in H0.
-      move/eqP in H2.
-      by subst.
-    }
-    { (* global *)
-      move/eqP in H1.
-      move/eqP in H4.
-      by subst.
-    }
-  - by rewrite <- H in H3.
-  - by rewrite <- H in H0.
+  eapply Forall2_function_eq; eauto.
+  move => x y z Heq1 Heq2; simpl in *.
+  unfold module_import_typing in *.
+  destruct x => /=; simpl in *.
+  destruct imp_desc; simpl in *; destruct y, z => //; remove_bools_options; by subst.
 Qed.
-
 
 Lemma module_typing_det m it1 et1 it2 et2:
   module_typing m it1 et1 ->
@@ -81,135 +381,71 @@ Proof.
   (* Function types *)
   assert (fts1 = fts2) as Heqfts.
   { clear - Hmft1 Hmft2.
-    apply list_eq.
-    move => i.
-    rewrite -> Forall2_lookup in Hmft1.
-    specialize (Hmft1 i).
-    rewrite -> Forall2_lookup in Hmft2.
-    specialize (Hmft2 i).
-    destruct (mod_funcs !! i) eqn: Hfli; inversion Hmft1; inversion Hmft2; subst => //=.
-    destruct m, modfunc_type, y, y0; simpl in *.
-    destruct H1 as [_ [Heqtf1 _]].
-    destruct H4 as [_ [Heqtf2 _]].
-    move/eqP in Heqtf1.
-    move/eqP in Heqtf2.
-    rewrite Heqtf1 in Heqtf2.
-    by rewrite Heqtf2.
+    eapply Forall2_function_eq; eauto.
+    move => x y z Heq1 Heq2; simpl in *.
+    unfold module_func_typing in *.
+    simpl in *.
+    destruct x, modfunc_type, y, z => /=; simpl in *.
+    destruct Heq1 as [_ [Heq1 _]].
+    destruct Heq2 as [_ [Heq2 _]].
+    remove_bools_options.
+    by rewrite - Heq1 Heq2.
   }
   subst.
 
   (* Global types *)
   assert (gts1 = gts2) as Heqgts.
   { clear - Hmgt1 Hmgt2.
-    apply list_eq.
-    move => i.
-    rewrite -> Forall2_lookup in Hmgt1.
-    specialize (Hmgt1 i).
-    rewrite -> Forall2_lookup in Hmgt2.
-    specialize (Hmgt2 i).
-    destruct (mod_globals !! i) eqn: Hgli; inversion Hmgt1; inversion Hmgt2; subst => //=.
-    destruct m, modglob_type, y, y0; simpl in *.
-    destruct H1 as [_ [Heqgt1 _]].
-    destruct H4 as [_ [Heqgt2 _]].
-    inversion Heqgt1.
-    inversion Heqgt2.
-    by subst.
+    eapply Forall2_function_eq; eauto.
+    move => x y z Heq1 Heq2; simpl in *.
+    unfold module_func_typing in *.
+    simpl in *.
+    destruct x, modglob_type, y, z => /=; simpl in *.
+    destruct Heq1 as [_ [Heq1 _]].
+    destruct Heq2 as [_ [Heq2 _]].
+    inversion Heq1; inversion Heq2; by subst. 
   }
   subst.
   
   f_equal.
+
   clear - Hmext1 Hmext2.
-  apply list_eq.
-  move => i.
-  rewrite -> Forall2_lookup in Hmext1.
-  specialize (Hmext1 i).
-  rewrite -> Forall2_lookup in Hmext2.
-  specialize (Hmext2 i).    
-  destruct (et1 !! i) eqn:Hetl1; destruct (et2 !! i) eqn:Hetl2; inversion Hmext1; inversion Hmext2; subst => //=.
-  - rewrite <- H in H2.
-    inversion H2; subst; clear H2.
-    destruct x; simpl in *.
-    unfold module_export_typing in *.
-    destruct modexp_desc; [destruct f | destruct t | destruct m | destruct g]; simpl in *; destruct e; destruct e0 => //=.
-    { (* func *)
-      move/andP in H1; destruct H1.
-      move/andP in H4; destruct H4.
-      destruct (nth_error _ n) => //.
-      move/eqP in H1.
-      move/eqP in H3.
-      by subst.
-    }
-    { (* table *)
-      move/andP in H1; destruct H1.
-      move/andP in H4; destruct H4.
-      destruct (nth_error _ n) => //.
-      move/eqP in H1.
-      move/eqP in H3.
-      by subst.
-    }
-    { (* memory *)
-      move/andP in H1; destruct H1.
-      move/andP in H4; destruct H4.
-      destruct (nth_error _ n) => //.
-      move/eqP in H1.
-      move/eqP in H3.
-      by subst.
-    }
-    { (* global *)
-      move/andP in H1; destruct H1.
-      move/andP in H4; destruct H4.
-      destruct (nth_error _ n) => //.
-      move/eqP in H1.
-      move/eqP in H3.
-      by subst.
-    }
-  - by rewrite <- H in H3.
-  - by rewrite <- H in H0.
+  eapply Forall2_function_eq; eauto.
+  move => x y z Heq1 Heq2; simpl in *.
+  unfold module_export_typing in *.
+  simpl in *.
+  destruct x, modexp_desc; [destruct f | destruct t | destruct m | destruct g]; destruct y, z; simpl in *; remove_bools_options; by subst => //.
 Qed.    
   
 End module_typing_det.
 
 Definition exp_default := MED_func (Mk_funcidx 0).
 
-Lemma insert_at_insert {T: Type} v n (l: list T):
-  n < length l ->
-  insert_at v n l = <[ n := v ]> l.
-Proof.
-  move : v n.
-  induction l; intros; simpl in H; destruct n => /=; try by inversion H.
-  - specialize (IHl v n).
-    unfold insert_at.
-    simpl.
-    f_equal.
-    rewrite <- IHl; last by lias.
-    by unfold insert_at.
-Qed.
-
-Definition ext_func_addrs := (map (fun x => match x with | Mk_funcidx i => i end)) ∘ ext_funcs.
-Definition ext_tab_addrs := (map (fun x => match x with | Mk_tableidx i => i end)) ∘ ext_tabs.
-Definition ext_mem_addrs := (map (fun x => match x with | Mk_memidx i => i end)) ∘ ext_mems.
-Definition ext_glob_addrs := (map (fun x => match x with | Mk_globalidx i => i end)) ∘ ext_globs.
+Definition ext_func_addrs := (map (fun x => match x with | Mk_funcidx i => i end)) \o ext_funcs.
+Definition ext_tab_addrs := (map (fun x => match x with | Mk_tableidx i => i end)) \o ext_tabs.
+Definition ext_mem_addrs := (map (fun x => match x with | Mk_memidx i => i end)) \o ext_mems.
+Definition ext_glob_addrs := (map (fun x => match x with | Mk_globalidx i => i end)) \o ext_globs.
 
 Lemma ext_func_addrs_aux l:
-  ext_func_addrs l = fmap (fun '(Mk_funcidx i) => i) (ext_funcs l).
+  ext_func_addrs l = map (fun '(Mk_funcidx i) => i) (ext_funcs l).
 Proof.
   by [].
 Qed.
 
 Lemma ext_tab_addrs_aux l:
-  ext_tab_addrs l = fmap (fun '(Mk_tableidx i) => i) (ext_tabs l).
+  ext_tab_addrs l = map (fun '(Mk_tableidx i) => i) (ext_tabs l).
 Proof.
   by [].
 Qed.
 
 Lemma ext_mem_addrs_aux l:
-  ext_mem_addrs l = fmap (fun '(Mk_memidx i) => i) (ext_mems l).
+  ext_mem_addrs l = map (fun '(Mk_memidx i) => i) (ext_mems l).
 Proof.
   by [].
 Qed.
 
 Lemma ext_glob_addrs_aux l:
-  ext_glob_addrs l = fmap (fun '(Mk_globalidx i) => i) (ext_globs l).
+  ext_glob_addrs l = map (fun '(Mk_globalidx i) => i) (ext_globs l).
 Proof.
   by [].
 Qed.
@@ -239,14 +475,14 @@ Lemma ext_funcs_lookup_exist (modexps: list module_export_desc) n fn:
   exists k, modexps !! k = Some (MED_func fn).
 Proof.
   move: n fn.
-  induction modexps; move => n tn Hextfunclookup => //=.
+  induction modexps; move => n tn Hextfunclookup; try by destruct n => //=.
   simpl in Hextfunclookup.
   destruct a => //. 
   { simpl in *.
-       destruct n; simpl in *; first by inversion Hextfunclookup; subst; exists 0.
-       apply IHmodexps in Hextfunclookup.
-       destruct Hextfunclookup as [k ?].
-       by exists (S k).
+    destruct n; simpl in *; first by inversion Hextfunclookup; subst; exists 0.
+    apply IHmodexps in Hextfunclookup.
+    destruct Hextfunclookup as [k ?].
+    by exists (S k).
   }
   all: simpl in *. 
   all: apply IHmodexps in Hextfunclookup.
@@ -259,7 +495,7 @@ Lemma ext_tabs_lookup_exist (modexps: list module_export_desc) n tn:
   exists k, modexps !! k = Some (MED_table tn).
 Proof.
   move: n tn.
-  induction modexps; move => n tn Hexttablookup => //=.
+  induction modexps; move => n tn Hexttablookup; try by destruct n => //=.
   simpl in Hexttablookup.
   destruct a => //. 
   2: { simpl in *.
@@ -279,7 +515,7 @@ Lemma ext_mems_lookup_exist (modexps: list module_export_desc) n mn:
   exists k, modexps !! k = Some (MED_mem mn).
 Proof.
   move: n mn.
-  induction modexps; move => n mn Hextmemlookup => //=.
+  induction modexps; move => n mn Hextmemlookup; try by destruct n => //=.
   simpl in Hextmemlookup.
   destruct a => //. 
   3: { simpl in *.
@@ -299,7 +535,7 @@ Lemma ext_globs_lookup_exist (modexps: list module_export_desc) n fn:
   exists k, modexps !! k = Some (MED_global fn).
 Proof.
   move: n fn.
-  induction modexps; move => n tn Hextgloblookup => //=.
+  induction modexps; move => n tn Hextgloblookup; try by destruct n => //=.
   simpl in Hextgloblookup.
   destruct a => //. 
   4: { simpl in *.
@@ -319,7 +555,7 @@ Lemma ext_funcs_lookup_exist_inv (modexps: list module_export_desc) n idx:
   exists k, ((ext_funcs modexps) !! k = Some idx).
 Proof.
   move : n idx.
-  induction modexps; move => n idx H => //=.
+  induction modexps; move => n idx H; try by destruct n => //=.
   destruct n; simpl in *.
   { inversion H; subst; by exists 0 => /=. }
   apply IHmodexps in H.
@@ -333,7 +569,7 @@ Lemma ext_tabs_lookup_exist_inv (modexps: list module_export_desc) n idx:
   exists k, ((ext_tabs modexps) !! k = Some idx).
 Proof.
   move : n idx.
-  induction modexps; move => n idx H => //=.
+  induction modexps; move => n idx H; try by destruct n => //=.
   destruct n; simpl in *.
   { inversion H; subst; by exists 0 => /=. }
   apply IHmodexps in H.
@@ -347,7 +583,7 @@ Lemma ext_mems_lookup_exist_inv (modexps: list module_export_desc) n idx:
   exists k, ((ext_mems modexps) !! k = Some idx).
 Proof.
   move : n idx.
-  induction modexps; move => n idx H => //=.
+  induction modexps; move => n idx H; try by destruct n => //=.
   destruct n; simpl in *.
   { inversion H; subst; by exists 0 => /=. }
   apply IHmodexps in H.
@@ -361,76 +597,13 @@ Lemma ext_globs_lookup_exist_inv (modexps: list module_export_desc) n idx:
   exists k, ((ext_globs modexps) !! k = Some idx).
 Proof.
   move : n idx.
-  induction modexps; move => n idx H => //=.
+  induction modexps; move => n idx H; try by destruct n => //=.
   destruct n; simpl in *.
   { inversion H; subst; by exists 0 => /=. }
   apply IHmodexps in H.
   destruct H as [k Hl].
   destruct a; try by exists k.
   by exists (S k).
-Qed.
-
-Definition gen_index offset len : list nat :=
-  imap (fun i x => i+offset+x) (repeat 0 len).
-
-Lemma gen_index_lookup offset len k:
-  k < len ->
-  (gen_index offset len) !! k = Some (offset + k).
-Proof.
-  move => Hlen.
-  unfold gen_index.
-  rewrite list_lookup_imap => /=.
-  eapply repeat_lookup with (x := 0) in Hlen.
-  rewrite Hlen.
-  simpl.
-  f_equal.
-  by lias.
-Qed.
-
-Lemma gen_index_lookup_Some n l i x:
-  (gen_index n l) !! i = Some x ->
-  x = n + i /\ i < l.
-Proof.
-  unfold gen_index.
-  move => Hl.
-  rewrite list_lookup_imap in Hl.
-  destruct (repeat _ _ !! i) eqn: Hrl => //.
-  simpl in Hl.
-  inversion Hl; subst; clear Hl.
-  apply repeat_lookup_Some in Hrl as [-> ?].
-  by lias.
-Qed.
- 
-Lemma gen_index_NoDup n l:
-  NoDup (gen_index n l).
-Proof.
-  apply NoDup_alt.
-  move => i j x Hli Hlj.
-  apply gen_index_lookup_Some in Hli as [-> ?].
-  apply gen_index_lookup_Some in Hlj as [? ?].
-  by lias.
-Qed.
-
-Lemma gen_index_length n len:
-  length (gen_index n len) = len.
-Proof.
-  unfold gen_index.
-  rewrite imap_length.
-  by rewrite repeat_length.
-Qed.
-
-Lemma gen_index_extend offset len:
-  gen_index offset (len+1) = gen_index offset len ++ [::offset+len].
-Proof.
-  unfold gen_index.
-  rewrite repeat_app => /=.
-  induction len => //=.
-  f_equal => //.
-  do 2 rewrite - fmap_imap.
-  rewrite IHlen.
-  rewrite fmap_app => /=.
-  repeat f_equal.
-  by lias.
 Qed.
 
 Section Host.
@@ -440,6 +613,7 @@ Variable host_function: eqType.
 Local Definition function_closure := function_closure host_function.
 Local Definition store_record := store_record host_function.
 
+Local Definition alloc_Xs := @alloc_Xs host_function.
 Local Definition alloc_funcs := alloc_funcs host_function.
 Local Definition alloc_tabs := alloc_tabs host_function.
 Local Definition alloc_mems := alloc_mems host_function.
@@ -456,185 +630,174 @@ Variable host_instance: host host_function.
 Local Definition reduce := @reduce host_function host_instance.
 
 Definition gen_func_instance mf inst : function_closure :=
-  let ft := nth match modfunc_type mf with
+  let ft := List.nth match modfunc_type mf with
                 | Mk_typeidx n => n
-                end (inst_types inst) (Tf [] []) in
+                end (inst_types inst) (Tf [::] [::]) in
   FC_func_native inst ft (modfunc_locals mf) (modfunc_body mf).
                 
+(* Proving relations between stores obtained by alloc_Xs *)
+Lemma alloc_Xs_IP {A B: Type} (f: store_record -> A -> store_record * B) s_init xs s_end ys (R: store_record -> store_record -> list A -> list B -> Prop) :
+  alloc_Xs _ _ f s_init xs = (s_end, ys) ->
+  (R s_init s_init [::] [::]) ->
+  (forall s s0 x xs' ys' s' y,
+    (s, y) = f s' x ->
+    R s0 s' xs' ys' ->
+    R s0 s (xs' ++ [::x]) (ys' ++ [::y])) ->
+  R s_init s_end xs ys.
+Proof.
+  move: s_init s_end ys.
+  induction xs using rev_ind => //=; move => s_init s_end ys Hallocxs Hinit IH; simpl in *.
+  - unfold alloc_Xs, instantiation_spec.alloc_Xs in Hallocxs.
+    simpl in Hallocxs.
+    by injection Hallocxs as ->; subst.
+  - unfold alloc_Xs, instantiation_spec.alloc_Xs in Hallocxs.
+    rewrite fold_left_app in Hallocxs.
+    simpl in Hallocxs.
+    
+    remember (fold_left _ xs _) as fold_res.
+    destruct fold_res as [s0 ys0].
+    remember (f s0 x) as sf.
+    destruct sf as [s' y'].
+    injection Hallocxs as ->; subst.
+    eapply IH; eauto.
+    apply IHxs; eauto.
+    unfold alloc_Xs, instantiation_spec.alloc_Xs.
+    by rewrite <- Heqfold_res.
+Qed.
 
 Lemma alloc_func_gen_index modfuncs ws inst ws' l:
   alloc_funcs ws modfuncs inst = (ws', l) ->
   map (fun x => match x with | Mk_funcidx i => i end) l = gen_index (length (s_funcs ws)) (length modfuncs) /\
-  ws'.(s_funcs) = ws.(s_funcs) ++ fmap (fun mf => gen_func_instance mf inst) modfuncs /\
+  ws'.(s_funcs) = ws.(s_funcs) ++ map (fun mf => gen_func_instance mf inst) modfuncs /\
   ws.(s_tables) = ws'.(s_tables) /\
   ws.(s_mems) = ws'.(s_mems) /\
   ws.(s_globals) = ws'.(s_globals).
 Proof.
-  unfold alloc_funcs, instantiation_spec.alloc_funcs, alloc_Xs.
-  generalize dependent l.
-  generalize dependent ws'.
-  generalize dependent ws.
-  induction modfuncs using List.rev_ind; move => ws ws' l Hallocfuncs.
-  - inversion Hallocfuncs; subst; clear Hallocfuncs.
-    simpl.
-    repeat split => //.
+  unfold alloc_funcs, instantiation_spec.alloc_funcs.
+  move => Halloc.
+  eapply alloc_Xs_IP with
+    (R := (fun s_i s_e xs ys => map _ ys = gen_index _ _ /\ _))
+    in Halloc; eauto => //=.
+  - unfold gen_index, imap => /=.
+    repeat split.
     by rewrite app_nil_r.
-  - rewrite fold_left_app in Hallocfuncs.
-    remember (fold_left _ modfuncs (ws,[])) as fold_res.
-    simpl in Hallocfuncs.
-    destruct fold_res as [ws0 l0].
-    symmetry in Heqfold_res.
-    unfold add_func in Hallocfuncs.
-    inversion Hallocfuncs; subst; clear Hallocfuncs.
-    rewrite map_app app_length /=.
-    rewrite gen_index_extend.
-    specialize (IHmodfuncs ws ws0 (rev l0)).
-    destruct IHmodfuncs as [? [? [? [? ?]]]]; first by rewrite Heqfold_res.
-    repeat split => //; try by eapply IHmodfuncs; rewrite Heqfold_res.
-    + rewrite H.
-      rewrite H0.
-      by rewrite app_length map_length.
-    + rewrite H0.
-      rewrite - app_assoc.
-      f_equal.
-      by rewrite -> list_fmap_app.
+  - move => s s0 x xs' ys' s' y Hallocx [Hys [Hcomp [? [? ?]]]].
+    unfold alloc_func, add_func in Hallocx; injection Hallocx as ->; subst => /=.
+    rewrite app_length map_app gen_index_extend Hys Hcomp => /=.
+    repeat split => //=.
+    + by rewrite app_length map_length.
+    + rewrite map_app.
+      unfold gen_func_instance => /=.
+      by rewrite app_assoc.
 Qed.
 
 Lemma alloc_tab_gen_index modtabtypes ws ws' l:
   alloc_tabs ws modtabtypes = (ws', l) ->
   map (fun x => match x with | Mk_tableidx i => i end) l = gen_index (length (s_tables ws)) (length modtabtypes) /\
-  ws'.(s_tables) = ws.(s_tables) ++ fmap (fun '{| tt_limits := {| lim_min := min; lim_max := maxo |} |} => {| table_data := repeat None (ssrnat.nat_of_bin min); table_max_opt := maxo |}) modtabtypes /\
+  ws'.(s_tables) = ws.(s_tables) ++ map (fun '{| tt_limits := {| lim_min := min; lim_max := maxo |} |} => {| table_data := repeat None (ssrnat.nat_of_bin min); table_max_opt := maxo |}) modtabtypes /\
   ws.(s_funcs) = ws'.(s_funcs) /\
   ws.(s_mems) = ws'.(s_mems) /\
   ws.(s_globals) = ws'.(s_globals).
 Proof.
-  unfold alloc_tabs, instantiation_spec.alloc_tabs, alloc_Xs.
-  generalize dependent l.
-  generalize dependent ws'.
-  generalize dependent ws.
-  induction modtabtypes using List.rev_ind; move => ws ws' l Halloc.
-  - inversion Halloc; subst; clear Halloc.
-    repeat split => //.
-    simpl.
+  unfold alloc_tabs, instantiation_spec.alloc_tabs.
+  move => Halloc.
+  eapply alloc_Xs_IP with
+    (R := (fun s_i s_e xs ys => map _ ys = gen_index _ _ /\ _))
+    in Halloc; eauto => //=.
+  - unfold gen_index, imap => /=.
+    repeat split.
     by rewrite app_nil_r.
-  - rewrite fold_left_app in Halloc.
-    remember (fold_left _ modtabtypes (ws,[])) as fold_res.
-    simpl in Halloc.
-    destruct fold_res as [ws0 l0].
-    symmetry in Heqfold_res.
-    unfold alloc_tab, add_table in Halloc.
-    destruct x => /=.
-    destruct tt_limits => /=.
-    specialize (IHmodtabtypes ws ws0 (rev l0)).
-    rewrite Heqfold_res in IHmodtabtypes.
-    inversion Halloc; subst; clear Halloc.
-    simpl in *.
-    rewrite map_app app_length /=.
-    rewrite gen_index_extend.
-    destruct IHmodtabtypes as [? [? [? [? ?]]]] => //.
-    repeat split => //.
-    + rewrite H.
-      rewrite H0.
-      by rewrite app_length map_length.
-    + rewrite H0.
-      rewrite - app_assoc.
-      f_equal.
-      by rewrite -> list_fmap_app => /=.
+  - move => s s0 x xs' ys' s' y Hallocx [Hys [Hcomp [? [? ?]]]].
+    unfold alloc_tab, add_table in Hallocx. destruct x as [[lim_min lim_max]]. injection Hallocx as ->; subst => /=.
+    rewrite app_length map_app gen_index_extend Hys Hcomp => /=.
+    repeat split => //=.
+    + by rewrite app_length map_length.
+    + rewrite map_app.
+      by rewrite app_assoc.
 Qed.
 
 Lemma alloc_mem_gen_index modmemtypes ws ws' l:
   alloc_mems ws modmemtypes = (ws', l) ->
   map (fun x => match x with | Mk_memidx i => i end) l = gen_index (length (s_mems ws)) (length modmemtypes) /\
-  ws'.(s_mems) = ws.(s_mems) ++ fmap (fun '{| lim_min := min; lim_max := maxo |} => {| mem_data := memory_list.mem_make #00%byte (page_size * min)%N; mem_max_opt := maxo |}) modmemtypes /\
+  ws'.(s_mems) = ws.(s_mems) ++ map (fun '{| lim_min := min; lim_max := maxo |} => {| mem_data := memory_list.mem_make #00%byte (page_size * min)%N; mem_max_opt := maxo |}) modmemtypes /\
   ws.(s_funcs) = ws'.(s_funcs) /\
   ws.(s_tables) = ws'.(s_tables) /\
   ws.(s_globals) = ws'.(s_globals).
 Proof.
-  unfold alloc_mems, instantiation_spec.alloc_mems, alloc_Xs.
-  generalize dependent l.
-  generalize dependent ws'.
-  generalize dependent ws.
-  induction modmemtypes using List.rev_ind; move => ws ws' l Halloc.
-  - inversion Halloc; subst; clear Halloc.
-    repeat split => //=.
+  unfold alloc_mems, instantiation_spec.alloc_mems.
+  move => Halloc.
+  eapply alloc_Xs_IP with
+    (R := (fun s_i s_e xs ys => map _ ys = gen_index _ _ /\ _))
+    in Halloc; eauto => //=.
+  - unfold gen_index, imap => /=.
+    repeat split.
     by rewrite app_nil_r.
-  - rewrite fold_left_app in Halloc.
-    remember (fold_left _ modmemtypes (ws,[])) as fold_res.
-    simpl in Halloc.
-    destruct fold_res as [ws0 l0].
-    symmetry in Heqfold_res.
-    unfold alloc_mem, add_mem in Halloc.
-    destruct x => /=.
-    specialize (IHmodmemtypes ws ws0 (rev l0)).
-    rewrite Heqfold_res in IHmodmemtypes.
-    inversion Halloc; subst; clear Halloc.
-    simpl in *.
-    rewrite map_app app_length /=.
-    rewrite gen_index_extend.
-    destruct IHmodmemtypes as [? [? [? [? ?]]]] => //.
-    repeat split => //.
-    + rewrite H.
-      rewrite H0.
-      by rewrite app_length fmap_length.
-    + rewrite H0.
-      rewrite - app_assoc.
-      f_equal.
-      by rewrite -> list_fmap_app => /=.
+  - move => s s0 x xs' ys' s' y Hallocx [Hys [Hcomp [? [? ?]]]].
+    unfold alloc_mem, add_mem in Hallocx. destruct x as [memid]. injection Hallocx as ->; subst => /=.
+    rewrite app_length map_app gen_index_extend Hys Hcomp => /=.
+    repeat split => //=.
+    + by rewrite app_length map_length.
+    + rewrite map_app.
+      by rewrite app_assoc.
+Qed.
+
+Lemma combine_snoc {T1 T2: Type}: forall (l1: list T1) (l2: list T2) lc x,
+  lc ++ [::x] = combine l1 l2 ->
+  length l1 = length l2 ->
+  exists l1' l2' a b,
+    (l1 = l1' ++ [::a] /\ l2 = l2' ++ [::b] /\ lc = combine l1' l2' /\ x = (a, b)).
+Proof.
+  induction l1 as [| a l1']; move => l2 lc x Hcomb Hlen; first by destruct lc.
+  destruct l2 as [|b l2'], lc as [|p lc'] => //; simpl in *; try by rewrite combine_nil in Hcomb.
+  - destruct l1', l2' => //; simpl in *.
+    injection Hcomb as ->.
+    by exists nil, nil, a, b.
+  - simpl in *.
+    injection Hlen as Hlen.
+    injection Hcomb as ->.
+    apply IHl1' in H => //.
+    destruct H as [l1'' [l2'' [a' [b' [-> [-> [-> ->]]]]]]].
+    by exists (a :: l1''), (b :: l2''), a', b'.
 Qed.
 
 Lemma alloc_glob_gen_index modglobs ws g_inits ws' l:
   length g_inits = length modglobs ->
   alloc_globs ws modglobs g_inits = (ws', l) ->
   map (fun x => match x with | Mk_globalidx i => i end) l = gen_index (length (s_globals ws)) (length modglobs) /\
-  ws'.(s_globals) = ws.(s_globals) ++ fmap (fun '({| modglob_type := gt; modglob_init := ge |}, v) => {| g_mut := gt.(tg_mut); g_val := v |} ) (combine modglobs g_inits) /\
+  ws'.(s_globals) = ws.(s_globals) ++ map (fun '({| modglob_type := gt; modglob_init := ge |}, v) => {| g_mut := gt.(tg_mut); g_val := v |} ) (combine modglobs g_inits) /\
   ws.(s_funcs) = ws'.(s_funcs) /\
   ws.(s_tables) = ws'.(s_tables) /\
   ws.(s_mems) = ws'.(s_mems).
 Proof.
-  unfold alloc_globs, instantiation_spec.alloc_globs, alloc_Xs.
-  generalize dependent l.
-  generalize dependent ws'.
-  generalize dependent ws.
-  generalize dependent g_inits.
-  induction modglobs using List.rev_ind; move => g_inits ws ws' l Hlen Halloc.
-  - inversion Halloc; subst; clear Halloc.
-    repeat split => //=.
+  unfold alloc_globs, instantiation_spec.alloc_globs.
+  move => Hgloblen Halloc.
+  move : Hgloblen.
+  remember (combine modglobs g_inits) as comb.
+  move : Heqcomb.
+  move : modglobs g_inits.
+  eapply alloc_Xs_IP with
+    (R := (fun s_i s_e xs ys => forall globs g_inits, xs = combine globs g_inits -> length g_inits = length globs -> map _ ys = gen_index _ _ /\ _))
+    in Halloc; eauto => //.
+  - unfold gen_index, imap => /=.
+    move => modglobs g_inits Hcomb Hgloblen.
+    destruct g_inits, modglobs => //=.
+    repeat split.
     by rewrite app_nil_r.
-  - destruct g_inits using List.rev_ind; first by destruct modglobs => /=.
-    repeat rewrite app_length in Hlen; simpl in Hlen.
-    repeat rewrite - cat_app in Halloc.
-    rewrite combine_app in Halloc; last by lias.
-    simpl in Halloc.
-    rewrite fold_left_app in Halloc.
-    lazymatch goal with
-    | _: context C [fold_left ?f (combine modglobs g_inits) (ws, [])] |- _ =>
-      remember (fold_left f (combine modglobs g_inits) (ws, [])) as fold_res
-    end.
-    destruct fold_res as [ws0 l0].
-    symmetry in Heqfold_res.
-    unfold alloc_glob, add_glob in Halloc.
-    simpl in Halloc.
-    inversion Halloc; subst; clear Halloc.
-    rewrite map_app app_length /=.
-    rewrite gen_index_extend.
-    specialize (IHmodglobs g_inits ws ws0 (rev l0)).
-    destruct IHmodglobs as [? [? [? [? ?]]]] => //.
-    + by lias.
-    + by rewrite Heqfold_res.
-    repeat split => //.
-    + rewrite H.
-      rewrite H0.
-      rewrite app_length fmap_length combine_length.
-      repeat f_equal.
+  - move => s s0 x xs' ys' s' y Hallocx Hind modglobs g_inits Hcomb Hgloblen.
+    apply combine_snoc in Hcomb; last by lias.
+    destruct Hcomb as [modglobs' [g_inits' [g [v [-> [-> [-> ->]]]]]]].
+    destruct (Hind modglobs' g_inits') as [Hys [Hcomp [? [? ?]]]] => //; clear Hind.
+    { repeat rewrite app_length in Hgloblen; simpl in Hgloblen. by lias. }
+    unfold alloc_glob, add_glob in Hallocx. injection Hallocx as ->; subst => /=.
+    rewrite app_length map_app gen_index_extend Hys Hcomp => /=.
+    repeat split => //=.
+    + rewrite app_length map_length combine_length.
+      do 3 f_equal.
+      repeat rewrite app_length in Hgloblen; simpl in Hgloblen.
       by lias.
-    + rewrite H0.
-      rewrite - app_assoc.
-      f_equal.
-      rewrite combine_app => /=.
-      rewrite -> list_fmap_app => /=.
-      repeat f_equal.
-      destruct x => //.
-      by lias.
+    + rewrite map_app.
+      rewrite app_assoc => /=.
+      by destruct g.
 Qed.
 
 Lemma init_tabs_preserve ws inst e_inits melem ws':
@@ -689,9 +852,9 @@ Proof.
   move : Himptype.
   move : t_imps fts gts.
   induction mod_imports; move => t_imps fts gts Himptype => //=.
-  - apply Forall2_nil_inv_l in Himptype as ->.
-    by simpl.
-  - destruct t_imps; first by apply Forall2_nil_inv_r in Himptype.
+  - apply Forall2_length in Himptype.
+    by destruct t_imps => //=.
+  - destruct t_imps; first by apply Forall2_length in Himptype.
     simpl in *.
     inversion Himptype; subst; clear Himptype.
     unfold module_import_typing in H2.
@@ -747,12 +910,9 @@ Proof.
     simpl in Hconst.
     move/andP in Hconst.
     destruct Hconst as [Hconst Hconsts].
-    eapply IHes in Hconsts => //.
-    f_equal.
+    eapply IHes in Hbet2 => //.
     assert (length t2 + 1 = length ts + length t2s) as Hlent2.
-    { rewrite <- app_length.
-      rewrite <- cat_app.
-      rewrite <- Heqt2.
+    { rewrite - app_length - cat_app - Heqt2.
       by lias.
     }
     unfold const_expr in Hconst.
@@ -775,7 +935,7 @@ Qed.
   
 Lemma const_exprs_impl tc es t:
   const_exprs tc es ->
-  be_typing tc es (Tf [] [::t]) ->
+  be_typing tc es (Tf [::] [::t]) ->
   exists e, es = [:: e] /\ const_expr tc e.
 Proof.
   move => Hconst Hbet.
@@ -791,7 +951,7 @@ Qed.
 Local Definition host_state := host_state host_instance.
 
 Lemma const_no_reduce (hs hs': host_state) s f v s' f' e':
-  reduce hs s f [AI_basic (BI_const v)] hs' s' f' e' ->
+  reduce hs s f [::AI_basic (BI_const v)] hs' s' f' e' ->
   False.
 Proof.
   move => Hred.
@@ -820,7 +980,7 @@ Qed.
 Local Definition reduce_trans := @reduce_trans host_function host_instance.
 
 Lemma reduce_trans_const hs1 s1 f1 v1 hs2 s2 f2 v2:
-  reduce_trans (hs1, s1, f1, [AI_basic (BI_const v1)]) (hs2, s2, f2, [AI_basic (BI_const v2)]) ->
+  reduce_trans (hs1, s1, f1, [::AI_basic (BI_const v1)]) (hs2, s2, f2, [::AI_basic (BI_const v2)]) ->
   v1 = v2.
 Proof.
   move => Hred.
@@ -833,8 +993,8 @@ Proof.
 Qed.
 
 Lemma reduce_get_global hs s f hs' s' f' i e:
-  reduce hs s f [AI_basic (BI_get_global i)] hs' s' f' e ->
-  exists v, sglob_val s (f_inst f) i = Some v /\ e = [AI_basic (BI_const v)].
+  reduce hs s f [::AI_basic (BI_get_global i)] hs' s' f' e ->
+  exists v, sglob_val s (f_inst f) i = Some v /\ e = [::AI_basic (BI_const v)].
 Proof.
   move => Hred.
   dependent induction Hred; subst; try by repeat destruct vcs => //.
@@ -865,7 +1025,7 @@ Proof.
 Qed.
     
 Lemma reduce_trans_get_global hs s f hs' s' f' i v:
-  reduce_trans (hs, s, f, [AI_basic (BI_get_global i)]) (hs', s', f', [AI_basic (BI_const v)]) ->
+  reduce_trans (hs, s, f, [::AI_basic (BI_get_global i)]) (hs', s', f', [::AI_basic (BI_const v)]) ->
   sglob_val s (f_inst f) i = Some v.
 Proof.
   move => Hred.
@@ -881,6 +1041,38 @@ Proof.
   destruct y as [[[??]?]?].
   by apply const_no_reduce in H.
 Qed.
+
+Lemma modglobs_const: forall tc modglobs gt,
+  Forall2 (module_glob_typing tc) modglobs gt ->
+  Forall (fun g => exists e, g.(modglob_init) = [::e] /\ const_expr tc e) modglobs.
+Proof.
+  move => tc modglobs. move: tc.
+  induction modglobs; move => tc gt Hall2; destruct gt => //=.
+  - by apply Forall2_length in Hall2.
+  - inversion Hall2 as [ | ???? Ha Hall2']; subst.
+    constructor.
+    + unfold module_glob_typing in Ha.
+      destruct a => /=; destruct Ha as [Hconst [-> Hbet]].
+      by apply const_exprs_impl in Hbet; eauto.
+    + by eapply IHmodglobs; eauto.
+Qed.
+
+(*
+Lemma modelems_const: forall tc modelems et,
+  Forall (module_elem_typing) modelems et ->
+  Forall (fun g => exists e, g.(modelem_init) = [::e] /\ const_expr tc e) modelems.
+Proof.
+  move => tc modglobs. move: tc.
+  induction modglobs; move => tc gt Hall2; destruct gt => //=.
+  - by apply Forall2_length in Hall2.
+  - inversion Hall2 as [ | ???? Ha Hall2']; subst.
+    constructor.
+    + unfold module_glob_typing in Ha.
+      destruct a => /=; destruct Ha as [Hconst [-> Hbet]].
+      by apply const_exprs_impl in Hbet; eauto.
+    + by eapply IHmodglobs; eauto.
+Qed.
+*)
 
 Local Definition instantiate_globals := instantiate_globals host_function host_instance.
 Local Definition instantiate_elem := instantiate_elem host_function host_instance.
@@ -899,48 +1091,29 @@ Proof.
   destruct m; simpl in *.
   destruct Hmt as [fts [gts [_ [_ [_ [Hmgt _]]]]]].
   assert (length gi1 = length gi2) as Hlen; first by (apply Forall2_length in Hgi1; apply Forall2_length in Hgi2; rewrite Hgi1 in Hgi2).
-  apply list_eq.
-  move => i.
-  destruct (gi1 !! i) as [v1 | ] eqn:Hg1; last first.
-  { destruct (gi2 !! i) eqn:Hg2 => //; by apply lookup_lt_Some in Hg2; apply lookup_ge_None in Hg1; lias. }
-  { destruct (gi2 !! i) as [v2 | ] eqn:Hg2 => //; last by apply lookup_lt_Some in Hg1; apply lookup_ge_None in Hg2; lias.
-    rewrite -> Forall2_lookup in Hgi1.
-    rewrite -> Forall2_lookup in Hgi2.
-    rewrite -> Forall2_lookup in Hmgt.
-    specialize (Hgi1 i).
-    specialize (Hgi2 i).
-    specialize (Hmgt i).
-    rewrite Hg1 in Hgi1.
-    rewrite Hg2 in Hgi2.
-    inversion Hgi1; subst; clear Hgi1.
-    inversion Hgi2; subst; clear Hgi2.
-    rewrite <- H0 in H.
-    inversion H; subst; clear H.
-    rewrite <- H0 in Hmgt.
-    inversion Hmgt; subst; clear Hmgt.
-    destruct x0.
-    unfold module_glob_typing in H4.
-    destruct H4 as [Hconst [-> Hbet]].
-    apply const_exprs_impl in Hbet => //.
-    destruct Hbet as [e [-> Hconste]].
-    unfold const_exprs, const_expr in Hconste.
-    destruct e => //; simpl in *.
-    { apply reduce_trans_get_global in H1.
-      apply reduce_trans_get_global in H3.
-      specialize (Hsgveq i0).
-      simpl in H1, H3.
-      move/andP in Hconst.
-      destruct Hconst as [Hconst _].
-      move/andP in Hconst.
-      destruct Hconst as [Hilen _].
-      move/ssrnat.ltP in Hilen.
-      rewrite <- Hsgveq in H3 => //.
-      by rewrite H3 in H1.
-    }
-    { apply reduce_trans_const in H1.
-      apply reduce_trans_const in H3.
-      by subst.
-    }
+
+  remember (Build_t_context _ _ _ _ _ _ _ _) as tc.
+  apply modglobs_const in Hmgt.
+
+  eapply Forall2_function_eq_cond; eauto => //.
+  move => x y z Hconst Heq1 Heq2.
+  simpl in *.
+
+  destruct x as [gt gi]; simpl in *.
+  destruct Hconst as [e [-> Hconst]]; simpl in *.
+  unfold const_expr in Hconst.
+  rewrite Heqtc in Hconst; simpl in Hconst.
+  destruct e; simpl in * => //; remove_bools_options.
+  { apply reduce_trans_get_global in Heq1.
+    apply reduce_trans_get_global in Heq2.
+    specialize (Hsgveq i).
+    rewrite Hsgveq in Heq1; last by move/ssrnat.ltP in H; lias.
+    rewrite Heq1 in Heq2.
+    by injection Heq2.
+  }
+  { apply reduce_trans_const in Heq1.
+    apply reduce_trans_const in Heq2.
+    by subst.
   }
 Qed.
 
@@ -956,40 +1129,26 @@ Proof.
   destruct m; simpl in *.
   destruct Hmt as [fts [gts [_ [_ [_ [_ [Hmet _]]]]]]].
   assert (length eo1 = length eo2) as Hlen; first by (apply Forall2_length in Heo1; apply Forall2_length in Heo2; rewrite Heo1 in Heo2).
-  apply list_eq.
-  move => i.
-  destruct (eo1 !! i) as [v1 | ] eqn:He1; last first.
-  { destruct (eo2 !! i) eqn:He2 => //; by apply lookup_lt_Some in He2; apply lookup_ge_None in He1; lias. }
-  { destruct (eo2 !! i) as [v2 | ] eqn:He2 => //; last by apply lookup_lt_Some in He1; apply lookup_ge_None in He2; lias.
-    rewrite -> Forall2_lookup in Heo1.
-    rewrite -> Forall2_lookup in Heo2.
-    rewrite -> Forall_lookup in Hmet.
-    specialize (Heo1 i).
-    specialize (Heo2 i).
-    specialize (Hmet i).
-    rewrite He1 in Heo1.
-    rewrite He2 in Heo2.
-    inversion Heo1; subst; clear Heo1.
-    inversion Heo2; subst; clear Heo2.
-    rewrite <- H0 in H.
-    inversion H; subst; clear H.
-    rewrite <- H0 in Hmet.
-    specialize (Hmet x0).
-    destruct x0, modelem_table; simpl in *.
-    destruct Hmet as [Hconst [Hbet [Hlen1 Hlen2]]] => //.
-    apply const_exprs_impl in Hbet => //.
-    destruct Hbet as [e [-> Hconste]].
-    unfold const_exprs, const_expr in Hconste.
-    destruct e => //; simpl in *.
-    { apply reduce_trans_get_global in H1.
-      apply reduce_trans_get_global in H3.
-      rewrite H1 in H3.
-      by inversion H3.
-    }
-    { apply reduce_trans_const in H1.
-      apply reduce_trans_const in H3.
-      subst; by inversion H1.
-    }
+
+  eapply Forall2_function_eq_cond; eauto => //.
+  move => x y z Hconst Heq1 Heq2.
+  simpl in *.
+
+  destruct x as [[et] eo ei]; simpl in *.
+  destruct Hconst as [Hconst [Hbet [Hilen Halllen]]].
+  apply const_exprs_impl in Hbet => //; clear Hconst.
+  destruct Hbet as [e [-> Hconst]].
+  unfold const_expr in Hconst; simpl in Hconst.
+  destruct e; simpl in * => //; remove_bools_options.
+  { apply reduce_trans_get_global in Heq1.
+    apply reduce_trans_get_global in Heq2.
+    rewrite Heq1 in Heq2.
+    by injection Heq2.
+  }
+  { apply reduce_trans_const in Heq1.
+    apply reduce_trans_const in Heq2.
+    rewrite Heq1 in Heq2.
+    by injection Heq2.
   }
 Qed.
 
@@ -1005,40 +1164,26 @@ Proof.
   destruct m; simpl in *.
   destruct Hmt as [fts [gts [_ [_ [_ [_ [_ [Hmdt _]]]]]]]].
   assert (length do1 = length do2) as Hlen; first by (apply Forall2_length in Hdo1; apply Forall2_length in Hdo2; rewrite Hdo1 in Hdo2).
-  apply list_eq.
-  move => i.
-  destruct (do1 !! i) as [v1 | ] eqn:Hd1; last first.
-  { destruct (do2 !! i) eqn:Hd2 => //; by apply lookup_lt_Some in Hd2; apply lookup_ge_None in Hd1; lias. }
-  { destruct (do2 !! i) as [v2 | ] eqn:Hd2 => //; last by apply lookup_lt_Some in Hd1; apply lookup_ge_None in Hd2; lias.
-    rewrite -> Forall2_lookup in Hdo1.
-    rewrite -> Forall2_lookup in Hdo2.
-    rewrite -> Forall_lookup in Hmdt.
-    specialize (Hdo1 i).
-    specialize (Hdo2 i).
-    specialize (Hmdt i).
-    rewrite Hd1 in Hdo1.
-    rewrite Hd2 in Hdo2.
-    inversion Hdo1; subst; clear Hdo1.
-    inversion Hdo2; subst; clear Hdo2.
-    rewrite <- H0 in H.
-    inversion H; subst; clear H.
-    rewrite <- H0 in Hmdt.
-    specialize (Hmdt x0).
-    destruct x0, moddata_data; simpl in *.
-    destruct Hmdt as [Hconst [Hbet Hleni]] => //.
-    apply const_exprs_impl in Hbet => //.
-    destruct Hbet as [e [-> Hconste]].
-    unfold const_exprs, const_expr in Hconste.
-    destruct e => //; simpl in *.
-    { apply reduce_trans_get_global in H1.
-      apply reduce_trans_get_global in H3.
-      rewrite H1 in H3.
-      by inversion H3.
-    }
-    { apply reduce_trans_const in H1.
-      apply reduce_trans_const in H3.
-      subst; by inversion H1.
-    }
+
+  eapply Forall2_function_eq_cond; eauto => //.
+  move => x y z Hconst Heq1 Heq2.
+  simpl in *.
+
+  destruct x as [[dm] d_o di]; simpl in *.
+  destruct Hconst as [Hconst [Hbet Hilen]].
+  apply const_exprs_impl in Hbet => //; clear Hconst.
+  destruct Hbet as [e [-> Hconst]].
+  unfold const_expr in Hconst; simpl in Hconst.
+  destruct e; simpl in * => //; remove_bools_options.
+  { apply reduce_trans_get_global in Heq1.
+    apply reduce_trans_get_global in Heq2.
+    rewrite Heq1 in Heq2.
+    by injection Heq2.
+  }
+  { apply reduce_trans_const in Heq1.
+    apply reduce_trans_const in Heq2.
+    rewrite Heq1 in Heq2.
+    by injection Heq2.
   }
 Qed.
 
@@ -1223,39 +1368,35 @@ Proof.
   move/eqP in Ham1; move/eqP in Ham2.
   assert (g_inits = g_inits') as Heqgi.
   {
-    eapply module_glob_init_det => //.
+    eapply module_glob_init_det; eauto => //.
     move => i Hilen.
     unfold sglob_val, sglob, sglob_ind => /=.
     repeat rewrite nth_error_lookup.
-    repeat rewrite map_fmap.
-    repeat rewrite list_lookup_fmap.
+    repeat rewrite map_map.
+    repeat rewrite list_lookup_map.
     remember ((ext_globs v_imps ++ idg') !! i) as gi.
     specialize (vt_imps_comp_len _ _ _ _ Hexttype) as Hcomplen.
     destruct Hcomplen as [_ [_ [_ Hglen]]].
-    rewrite lookup_app in Heqgi.
     rewrite <- Hglen in Hilen.
-    destruct (ext_globs v_imps !! i) eqn:Hgvi; last by apply lookup_ge_None in Hgvi; lias.
-    subst gi.
-    simpl.
+    rewrite nth_error_app1 in Heqgi => //.
+    destruct gi as [g |]; symmetry in Heqgi; last by rewrite -> nth_error_None in Heqgi; lias.
     destruct g.
     assert (n < length (s_globals s)) as Hnlen.
     { unfold module_typing in Hmt.
       destruct m; simpl in *.
       destruct Hmt as [fts [gts [_ [_ [_ [_ [_ [_ [_ [Hit _]]]]]]]]]].
-      rewrite -> Forall2_lookup in Hexttype.
-      apply ext_globs_lookup_exist in Hgvi.
-      destruct Hgvi as [k Hvi].
-      specialize (Hexttype k).
-      rewrite Hvi in Hexttype.
+      apply ext_globs_lookup_exist in Heqgi as [k Hvi].
+      eapply Forall2_lookup in Hexttype; eauto.
+      destruct Hexttype as [y [Hnth Hexttype]].
+      Search n.
       inversion Hexttype; subst; clear Hexttype.
-      inversion H1; subst; clear H1.
-      by move/ssrnat.ltP in H2.
+      by move/ssrnat.ltP in H0.
     }
     subst s_res1 s_res2 => /=.
-    repeat rewrite nth_error_lookup.
-    repeat rewrite lookup_app.
-    destruct (s_globals s !! n) eqn:Hsgn => //=.
-    exfalso. apply lookup_ge_None in Hsgn. by lias.
+    rewrite Coqlib.list_map_nth => /=.
+    rewrite nth_error_app1 => //.
+    rewrite Heqgi => /=.
+    by repeat rewrite nth_error_app1 => //.
   }
   split => //; last by subst.
 Qed.
@@ -1278,7 +1419,7 @@ Proof.
   inversion Hvteq; subst; clear Hvteq.
 
   (* Instance, alloc_module store, and exports *)
-  eapply alloc_module_det in Hallocmodule1 => //.
+  eapply alloc_module_det in Hallocmodule1; eauto => //.
   3: { by apply Forall2_length in Hinstglob1. }
   2: { by apply Forall2_length in Hinstglob2. }
 
@@ -1293,10 +1434,10 @@ Proof.
 
   (* Final store *)
   assert (e_offs1 = e_offs2) as Heoffeq.
-  { by eapply module_elem_init_det. }
+  { by eapply module_elem_init_det; eauto. }
   
   assert (d_offs1 = d_offs2) as Hdoffeq.
-  { by eapply module_data_init_det. }
+  { by eapply module_data_init_det; eauto. }
 
   subst.
   move/eqP in Hws1.
